`p[j] != *`,如果` i && s[i] == p[j] || p[j] == ?`  `f[i][j] = f[i - 1][j - 1]`

 

`p[j] == *`

`f[i][j] = f[i][j - 1] || f[i - 1][j - 1] || f[i - 2][j - 1]`

`f[i - 1][j] = f[i - 1][j - 1] || f[ i - 2][j - 1] || f[i - 3][j - 1]`

所以`f[i][j] = f[i][j - 1] | f[i - 1][j]`

```c++
class Solution {
public:
    bool isMatch(string s, string p) {
        int n = s.size(), m = p.size();
        vector<vector<bool>> f(n + 1, vector<bool>(m + 1));
        s = ' ' + s, p = ' ' + p;
        f[0][0] = true;
        for(int i = 0; i <= n; i ++)
        {
            for(int j = 1; j <= m; j ++)
            {
                if(i && (s[i] == p[j] || p[j] == '?')) f[i][j] = f[i - 1][j - 1];
                else if(p[j] == '*')
                {
                    f[i][j] = f[i][j - 1];
                    if(i) f[i][j] = f[i][j] | f[i - 1][j];
                }
            }
        }
        return f[n][m];
    }
};
```

